State.thy
@@ -26,6 +26,14 @@ definition wp :: "'b pred \<Rightarrow> 'b rpred \<Rightarrow> 'b pred \<Rightar
   where "wp pre post Q \<equiv>
     pre \<inter> {m. (\<forall>m'. (m,m') \<in> post \<longrightarrow> m' \<in> Q) \<and> (\<exists>m'. (m,m') \<in> post)}"
 
+lemma wp_rel_partial:
+  "wp pre post Q = pre \<inter> Domain post \<inter> {m. (\<forall>m'. (m,m') \<in> post \<longrightarrow> m' \<in> Q)}"
+unfolding wp_def by auto
+
+lemma wp_rel:
+  "wp pre post Q = pre \<inter> Domain post \<inter> -(post\<inverse> `` (-Q))"
+unfolding wp_def by auto
+
 text \<open>Guarantee check for a pre-condition and post-relation\<close>
 definition guar :: "'b pred \<Rightarrow> 'b rpred \<Rightarrow> 'b rpred \<Rightarrow> bool"
   where "guar pre post G \<equiv> {(m,m'). m \<in> pre \<and> (m,m') \<in> post} \<subseteq> G"
